Core/LinFacts.v
@@ -1,25 +1,27 @@
 From LHL.Core Require Import
-    Program
-    Specs
-    Traces
-    Linearizability.
+  Program
+  Specs
+  Traces
+  Linearizability
+  VCompFacts
+  RefinesFacts
+  Tensor.
 
-From LHL.Core Require Import
-    VCompFacts
-    RefinesFacts.
+From LHL.Util Require Import
+  TransUtil
+  Tactics.
 
 (* Observational Refinement *)
 Theorem lin_obs_ref {E F} : 
-    forall (spec' spec : Spec E) (impl : Impl E F) ,
-        Lin spec' spec -> 
-        layerRefines (spec' :> impl) (spec :> impl).
-Proof.
-    intros.
-    apply (mkLayer_monotonic _ _ impl) in H.
-    assert (H' := layerRefines_VComp_assoc spec idImpl impl).
-    rewrite obj_VComp_assoc in H'.
-    assert (ID_EUTT := idImpl_is_identity_l impl).
-    assert (H'' := eutt_layerRefines spec _ _ ID_EUTT).
-    eapply layerRefines_trans. eapply layerRefines_trans.
-    apply H. apply H'. apply H''.
+  forall (spec' spec : Spec E) (impl : Impl E F) ,
+  Lin spec' spec -> 
+  layerRefines (spec' :> impl) (spec :> impl).
+intros.
+apply (mkLayer_monotonic _ _ impl) in H.
+assert (H' := layerRefines_VComp_assoc spec idImpl impl).
+rewrite obj_VComp_assoc in H'.
+assert (ID_EUTT := idImpl_is_identity_l impl).
+assert (H'' := eutt_layerRefines spec _ _ ID_EUTT).
+eapply layerRefines_trans. eapply layerRefines_trans.
+apply H. apply H'. apply H''.
 Qed.
