Examples/FAISpec.v
@@ -6,13 +6,13 @@ From LHL.Core Require Import
 Variant FAISig : ESig :=
 | FAI : FAISig nat.
 
-Variant FAIState :=
-| FAICalled (i : ThreadName) (n : nat)
-| FAIIdle (n : nat).
+Definition FAIState : Type := nat * option ThreadName.
+Definition FAIIdle n : FAIState := (n, None).
+Definition FAIRan i n : FAIState := (n, Some i).
 
 Variant FAIStep : FAIState -> ThreadEvent FAISig -> FAIState -> Prop :=
-| FAICall i n : FAIStep (FAIIdle n) (i, CallEv FAI) (FAICalled i n)
-| FAIRet i n : FAIStep (FAICalled i n) (i, RetEv FAI n) (FAIIdle (S n)).
+| FAICall i n : FAIStep (FAIIdle n) (i, CallEv FAI) (FAIRan i n)
+| FAIRet i n : FAIStep (FAIRan i n) (i, RetEv FAI n) (FAIIdle (S n)).
 
 Definition faiSpec : Spec FAISig := {|
   State := FAIState;
