Examples/VarSpec.v
@@ -9,39 +9,62 @@ From LHL.Util Require Import
 Variant VarSig {S} : ESig :=
 | SetVar : S -> VarSig unit
 | GetVar : VarSig S
-| ClearVar : VarSig S.
+| ClrVar : VarSig unit.
 Arguments VarSig : clear implicits.
+
+Record VarPend {S} := MkVarPend {
+  VarRetTy : Type;
+  VarCall : VarSig S VarRetTy
+}.
+Arguments VarPend : clear implicits.
+Arguments MkVarPend {S}.
 
 Variant VarValue {S} :=
 | VarUnset
-| VarIdle (s : S)
-| VarSetCalled (s : S)
-| VarGetCalled (s : S).
+| VarSet (s : S) (m : option (VarPend S)).
 Arguments VarValue : clear implicits.
+
+Definition VarIdle {S} (s : S) := VarSet s None.
+Definition VarSetRan {S} (s t : S) :=
+  VarSet s (Some (MkVarPend _ (SetVar t))).
+Definition VarGetRan {S} (s : S) :=
+  VarSet s (Some (MkVarPend _ GetVar)).
+Definition VarClrRan {S} (s : S) :=
+  VarSet s (Some (MkVarPend _ ClrVar)).
 
 Definition VarState S := ThreadName -> VarValue S.
 
 Variant VarStep {S} : VarState S -> ThreadEvent (VarSig S) -> VarState S -> Prop :=
-| VarCallSet i m m' t :
-    m i = VarUnset ->
-    m' i = VarSetCalled t ->
+| VarCallSet i m m' s t :
+    m i = VarIdle s ->
+    m' i = VarSetRan s t ->
     differ_pointwise m m' i ->
     VarStep m (i, CallEv (SetVar t)) m'
-| VarRetSet i m m' s :
-    m i = VarSetCalled s ->
-    m' i = VarIdle s ->
+| VarRetSet i m m' s t :
+    m i = VarSetRan s t ->
+    m' i = VarIdle t ->
     differ_pointwise m m' i ->
-    VarStep m (i, RetEv (SetVar s) tt) m'
+    VarStep m (i, RetEv (SetVar t) tt) m'
 | VarCallGet i m m' s :
     m i = VarIdle s ->
-    m' i = VarGetCalled s ->
+    m' i = VarGetRan s ->
     differ_pointwise m m' i ->
     VarStep m (i, CallEv GetVar) m'
 | VarRetGet i m m' s :
-    m i = VarGetCalled s ->
+    m i = VarGetRan s ->
     m' i = VarIdle s ->
     differ_pointwise m m' i ->
-    VarStep m (i, RetEv GetVar s) m'.
+    VarStep m (i, RetEv GetVar s) m'
+| VarInvClr i m m' s :
+    m i = VarIdle s ->
+    m' i = VarClrRan s ->
+    differ_pointwise m m' i ->
+    VarStep m (i, CallEv ClrVar) m'
+| VarRetClr i m m' s :
+    m i = VarClrRan s ->
+    m' i = VarUnset ->
+    differ_pointwise m m' i ->
+    VarStep m (i, RetEv ClrVar tt) m'.
 
 Definition varSpec S : Spec (VarSig S) := {|
   State := VarState S;
